examples/dsls/mini_steel/Pulse.Steel.Wrapper.fsti
@@ -214,3 +214,8 @@ val read_atomic (r:R.ref u32) (n:erased u32) (p:perm)
   : stt_atomic u32 emp_inames
                (R.pts_to r p n)
                (fun _ -> R.pts_to r p n)
+
+val read_explicit (r:R.ref u32) (n:erased u32) (p:perm)
+  : stt u32
+        (R.pts_to r p n)
+        (fun _ -> R.pts_to r p n)
